candle/standard/monadic/holKernelProofScript.sml
@@ -35,7 +35,7 @@ val REPLICATE_11 = Q.prove(
   `!m n x. (REPLICATE n x = REPLICATE m x) = (m = n)`,
   Induct \\ Cases \\ SRW_TAC [] [rich_listTheory.REPLICATE]);
 
-Overload impossible_term = ``holSyntax$Comb (Var (strlit "x") Bool) (Var (strlit "x") Bool)``
+Overload impossible_term = ``holSyntax$Comb (Var (implode "x") Bool) (Var (implode "x") Bool)``
 
 (* ------------------------------------------------------------------------- *)
 (* case_eq theorems                                                          *)
@@ -123,7 +123,7 @@ val CONTEXT_std_sig = Q.prove(
 
 val CONTEXT_fun = Q.prove(
   `CONTEXT defs ⇒
-      ∀a. MEM (strlit"fun",a) (type_list defs) ⇔ (a = 2)`,
+      ∀a. MEM (implode"fun",a) (type_list defs) ⇔ (a = 2)`,
   rw[] >> imp_res_tac CONTEXT_ALL_DISTINCT >>
   imp_res_tac CONTEXT_std_sig >>
   fs[is_std_sig_def] >>
@@ -149,7 +149,7 @@ val TERM = Q.prove(
 
 val TYPE_Fun = Q.prove(
   `CONTEXT defs ∧ TYPE defs ty1 /\ TYPE defs ty2 ==>
-    TYPE defs (Tyapp (strlit "fun") [ty1;ty2])`,
+    TYPE defs (Tyapp (implode "fun") [ty1;ty2])`,
   rw[TYPE_def,type_ok_def] >>
   imp_res_tac CONTEXT_fun >>
   METIS_TAC[ALOOKUP_ALL_DISTINCT_MEM,CONTEXT_ALL_DISTINCT]);
@@ -320,7 +320,7 @@ Theorem mk_type_thm:
    !tyop args s z s'.
       STATE defs s /\ EVERY (TYPE defs) args /\
       (mk_type (tyop,args) s = (z,s')) ==> (s' = s) /\
-      ((tyop = (strlit "fun")) /\ (LENGTH args = 2) ==> ?i. z = Success i) /\
+      ((tyop = (implode "fun")) /\ (LENGTH args = 2) ==> ?i. z = Success i) /\
       !i. (z = Success i) ==> TYPE defs i /\ (i = Tyapp tyop args)
 Proof
   SIMP_TAC std_ss [mk_type_def,try_def,st_ex_bind_def,otherwise_def]
@@ -401,7 +401,7 @@ Theorem mk_fun_ty_thm:
    !ty1 ty2 s z s'.
       STATE defs s /\ EVERY (TYPE defs) [ty1;ty2] /\
       (mk_fun_ty ty1 ty2 s = (z,s')) ==> (s' = s) /\
-      ?i. (z = Success i) /\ (i = Tyapp (strlit "fun") [ty1;ty2]) /\ TYPE defs i
+      ?i. (z = Success i) /\ (i = Tyapp (implode "fun") [ty1;ty2]) /\ TYPE defs i
 Proof
   SIMP_TAC std_ss [mk_fun_ty_def] \\ REPEAT STRIP_TAC
   \\ IMP_RES_TAC mk_type_thm \\ FULL_SIMP_TAC (srw_ss()) []
@@ -411,7 +411,7 @@ QED
 (* Verification of term functions                                            *)
 (* ------------------------------------------------------------------------- *)
 
-Overload aty[local] = ``(Tyvar (strlit "A")):type``
+Overload aty[local] = ``(Tyvar (implode "A")):type``
 
 val get_const_type_thm = Q.prove(
   `!name s z s'.
@@ -427,10 +427,10 @@ val term_type_def = Define `
     case tm of
       Var _ ty => ty
     | Const _ ty => ty
-    | Comb s _ => (case term_type s of Tyapp (strlit "fun") (_::ty1::_) => ty1
-                                    | _ => Tyvar (strlit ""))
-    | Abs (Var _ ty) t => Tyapp (strlit "fun") [ty; term_type t]
-    | _ => Tyvar (strlit "")`
+    | Comb s _ => (case term_type s of Tyapp (implode "fun") (_::ty1::_) => ty1
+                                    | _ => Tyvar (implode ""))
+    | Abs (Var _ ty) t => Tyapp (implode "fun") [ty; term_type t]
+    | _ => Tyvar (implode "")`
 
 val term_type = Q.prove(
   `!defs tm. CONTEXT defs ∧ TERM defs tm ==>
@@ -503,7 +503,7 @@ val type_of_thm = Q.prove(
     \\ IMP_RES_TAC TERM \\ FULL_SIMP_TAC (srw_ss()) []
     \\ ONCE_REWRITE_TAC [st_ex_bind_def]
     \\ FULL_SIMP_TAC (srw_ss()) [dest_type_def]
-    \\ reverse (sg `?ty1 ty2. term_type t = Tyapp (strlit "fun") [ty1;ty2]`) THEN1
+    \\ reverse (sg `?ty1 ty2. term_type t = Tyapp (implode "fun") [ty1;ty2]`) THEN1
      (FULL_SIMP_TAC (srw_ss()) [st_ex_return_def,codomain_def]
       \\ IMP_RES_TAC TYPE \\ ASM_SIMP_TAC (srw_ss()) [EVERY_DEF,Once term_type_def])
     \\ fs[TERM_def,term_ok_def] >>
@@ -739,9 +739,9 @@ QED
 
 val get_const_type_Equal = Q.prove(
   `STATE defs s ==>
-    (get_const_type (strlit "=") s = (Success (Fun aty (Fun aty Bool)),s))`,
+    (get_const_type (implode "=") s = (Success (Fun aty (Fun aty Bool)),s))`,
   SIMP_TAC std_ss [STATE_def]
-  \\ Cases_on `get_const_type (strlit "=") s`
+  \\ Cases_on `get_const_type (implode "=") s`
   \\ IMP_RES_TAC get_const_type_thm \\ REPEAT STRIP_TAC >>
   imp_res_tac CONTEXT_std_sig >>
   imp_res_tac CONTEXT_ALL_DISTINCT >>
@@ -755,17 +755,17 @@ val get_const_type_Equal = Q.prove(
 
 val mk_const_eq = Q.prove(
   `STATE defs s ==>
-    (mk_const ((strlit "="),[]) s =
-     (Success (Const (strlit "=") (Fun aty (Fun aty Bool))),s))`,
+    (mk_const ((implode "="),[]) s =
+     (Success (Const (implode "=") (Fun aty (Fun aty Bool))),s))`,
   SIMP_TAC std_ss [mk_const_def,st_ex_bind_def,try_def,otherwise_def]
   \\ REPEAT STRIP_TAC \\ IMP_RES_TAC get_const_type_Equal
   \\ FULL_SIMP_TAC (srw_ss()) [st_ex_return_def]
   \\ EVAL_TAC);
 
 val mk_eq_lemma = Q.prove(
-  `inst [(term_type x,aty)] (Const (strlit "=") (Fun aty (Fun aty Bool))) s =
+  `inst [(term_type x,aty)] (Const (implode "=") (Fun aty (Fun aty Bool))) s =
     ex_return
-        (Const (strlit "=")
+        (Const (implode "=")
            (Fun (term_type x) (Fun (term_type x) Bool))) s`,
   NTAC 10 (SIMP_TAC (srw_ss()) [Once inst_def, Once inst_aux_def, Once LET_DEF])
   \\ NTAC 50 (SIMP_TAC (srw_ss()) [Once type_subst_def,LET_DEF, Once mk_vartype_def,
@@ -777,7 +777,7 @@ Theorem mk_eq_thm:
     (s' = s) /\
     (!t. (res = Failure t) ==> ((term_type x) <> (term_type y))) /\
     !t. (res = Success t) ==>
-    (t = Comb (Comb (Const (strlit "=") (Fun (term_type x)
+    (t = Comb (Comb (Const (implode "=") (Fun (term_type x)
                                (Fun (term_type x) Bool))) x) y) /\
     TERM defs t
 Proof
@@ -788,18 +788,18 @@ Proof
   \\ FULL_SIMP_TAC std_ss [] \\ STRIP_TAC \\ FULL_SIMP_TAC (srw_ss()) []
   \\ IMP_RES_TAC mk_const_eq \\ FULL_SIMP_TAC (srw_ss()) []
   \\ FULL_SIMP_TAC (srw_ss()) [mk_eq_lemma,st_ex_return_def]
-  \\ Cases_on `mk_comb (Const (strlit "=") (Fun (term_type x)
+  \\ Cases_on `mk_comb (Const (implode "=") (Fun (term_type x)
                                   (Fun (term_type x) Bool)),x) s`
-  \\ sg `TERM defs (Const (strlit "=") (Fun (term_type x)
+  \\ sg `TERM defs (Const (implode "=") (Fun (term_type x)
                            (Fun (term_type x) Bool)))` THEN1
    (IMP_RES_TAC term_type >>
     IMP_RES_TAC CONTEXT_std_sig
     \\ FULL_SIMP_TAC (srw_ss()) [TERM_def] >>
     simp[term_ok_def] >> fs[is_std_sig_def,type_ok_def,TYPE_def] >>
     rfs[] >>
-    qexists_tac`[(typeof x,Tyvar(strlit "A"))]` >>
+    qexists_tac`[(typeof x,Tyvar(implode "A"))]` >>
     simp[REV_ASSOCD] )
-  \\ Q.ABBREV_TAC `eq = (Const (strlit "=") (Fun (term_type x) (Fun (term_type x) Bool)))`
+  \\ Q.ABBREV_TAC `eq = (Const (implode "=") (Fun (term_type x) (Fun (term_type x) Bool)))`
   \\ MP_TAC (mk_comb_thm |> Q.INST [`f`|->`eq`,`a`|->`x`,`res`|->`q`,`s1`|->`r`])
   \\ FULL_SIMP_TAC std_ss [] \\ STRIP_TAC
   \\ ONCE_REWRITE_TAC [EQ_SYM_EQ]
@@ -807,7 +807,7 @@ Proof
    (Q.UNABBREV_TAC `eq` \\ FULL_SIMP_TAC std_ss [mk_comb_def,st_ex_bind_def]
     \\ IMP_RES_TAC (Q.SPEC `y` type_of_thm)
     \\ Q.PAT_X_ASSUM `type_of x s = (Success (term_type x),s)` ASSUME_TAC
-    \\ FULL_SIMP_TAC (srw_ss()) [EVAL ``term_type (Const (strlit "=") ty)``,st_ex_return_def])
+    \\ FULL_SIMP_TAC (srw_ss()) [EVAL ``term_type (Const (implode "=") ty)``,st_ex_return_def])
   \\ FULL_SIMP_TAC std_ss []
   \\ Cases_on `mk_comb (Comb eq x,y) s`
   \\ MP_TAC (mk_comb_thm |> Q.INST [`f`|->`Comb eq x`,`a`|->`y`,
@@ -818,7 +818,7 @@ Proof
   \\ Q.UNABBREV_TAC `eq` \\ FULL_SIMP_TAC std_ss [mk_comb_def,st_ex_bind_def]
   \\ IMP_RES_TAC (Q.SPEC `y` type_of_thm)
   \\ Q.PAT_X_ASSUM `type_of x s = (Success (term_type x),s)` ASSUME_TAC
-  \\ FULL_SIMP_TAC (srw_ss()) [EVAL ``term_type (Const (strlit "=") ty)``,st_ex_return_def,
+  \\ FULL_SIMP_TAC (srw_ss()) [EVAL ``term_type (Const (implode "=") ty)``,st_ex_return_def,
          ``term_type (Comb x y)`` |> SIMP_CONV (srw_ss()) [Once term_type_def],
          ``type_of (Comb x y)`` |> SIMP_CONV (srw_ss()) [Once type_of_def],
          ``type_of (Const x y)`` |> SIMP_CONV (srw_ss()) [Once type_of_def],
@@ -826,7 +826,7 @@ Proof
 QED
 
 val TERM_Eq_x = Q.prove(
-  `STATE defs s /\ TERM defs (Comb (Const (strlit "=") ty) x) ==>
+  `STATE defs s /\ TERM defs (Comb (Const (implode "=") ty) x) ==>
     (Fun (typeof x) (Fun (typeof x) Bool) = ty)`,
   rw[TERM_def,STATE_def] >>
   fs[term_ok_def] >>
@@ -849,13 +849,13 @@ val MAP_EQ_2_SYM = Q.prove(
   `([x;y] = MAP f l) ⇔ (MAP f l = [x;y])`,METIS_TAC[])
 
 val Equal_type = Q.prove(
-  `STATE defs s ∧ TERM defs (Const (strlit "=") ty) ==> ?a. ty = Fun a (Fun a Bool)`,
+  `STATE defs s ∧ TERM defs (Const (implode "=") ty) ==> ?a. ty = Fun a (Fun a Bool)`,
   rw[STATE_def,TERM_def] >>
   imp_res_tac CONTEXT_std_sig >>
   fs[is_std_sig_def,term_ok_def])
 
 val Equal_type_IMP = Q.prove(
-  `STATE defs s ∧ TERM defs (Comb (Const (strlit "=") (Fun a' (Fun a' Bool))) ll) ==>
+  `STATE defs s ∧ TERM defs (Comb (Const (implode "=") (Fun a' (Fun a' Bool))) ll) ==>
     (typeof ll = a')`,
   simp[TERM_Comb] >> strip_tac >>
   imp_res_tac TERM_Eq_x >>
@@ -1121,7 +1121,7 @@ val type_of_state = Q.prove(
         try_def,otherwise_def,get_type_arity_def,
         get_the_type_constants_def,raise_Fail_def,st_ex_return_def]
   \\ STRIP_ASSUME_TAC (assoc_state |> ISPEC ``s.the_type_constants``
-        |> ISPEC ``strlit"fun"``) \\ FULL_SIMP_TAC std_ss []
+        |> ISPEC ``implode"fun"``) \\ FULL_SIMP_TAC std_ss []
   \\ Cases_on `r` \\ FULL_SIMP_TAC (srw_ss()) []
   \\ SRW_TAC [] []);
 
@@ -1565,9 +1565,9 @@ Proof
   \\ BasicProvers.EVERY_CASE_TAC
   \\ FULL_SIMP_TAC (srw_ss()) [raise_Fail_def]
   \\ SRW_TAC [] [st_ex_bind_def] \\ IMP_RES_TAC THM
-  \\ Q.MATCH_ASSUM_RENAME_TAC `TERM defs (Comb (Comb (Const (strlit "=") h1) ll) m1)`
+  \\ Q.MATCH_ASSUM_RENAME_TAC `TERM defs (Comb (Comb (Const (implode "=") h1) ll) m1)`
   \\ POP_ASSUM MP_TAC
-  \\ Q.MATCH_ASSUM_RENAME_TAC `TERM defs (Comb (Comb (Const (strlit "=") h2) m2) rr)`
+  \\ Q.MATCH_ASSUM_RENAME_TAC `TERM defs (Comb (Comb (Const (implode "=") h2) m2) rr)`
   \\ REPEAT STRIP_TAC \\ IMP_RES_TAC TERM \\ Cases_on `mk_eq (ll,rr) s`
   \\ MP_TAC (mk_eq_thm |> Q.INST [`x`|->`ll`,`y`|->`rr`,`res`|->`q`,`s'`|->`r`])
   \\ FULL_SIMP_TAC std_ss [] \\ IMP_RES_TAC TERM
@@ -1671,7 +1671,7 @@ Proof
   IMP_RES_TAC map_type_of_state >> var_eq_tac >>
   every_case_tac >> fs[] >>
   rpt var_eq_tac >> simp[] >>
-  qspecl_then[`strlit"bool"`,`[]`,`s`]mp_tac mk_type_thm >>
+  qspecl_then[`implode"bool"`,`[]`,`s`]mp_tac mk_type_thm >>
   simp[] >> strip_tac >>
   rpt var_eq_tac >> simp[] >>
   fs[THM_def] >>
@@ -1709,9 +1709,9 @@ Proof
   \\ BasicProvers.EVERY_CASE_TAC
   \\ FULL_SIMP_TAC (srw_ss()) [raise_Fail_def]
   \\ SRW_TAC [] [st_ex_bind_def] \\ IMP_RES_TAC THM
-  \\ Q.MATCH_ASSUM_RENAME_TAC `TERM defs (Comb (Comb (Const (strlit "=") h1) f1) f2)`
+  \\ Q.MATCH_ASSUM_RENAME_TAC `TERM defs (Comb (Comb (Const (implode "=") h1) f1) f2)`
   \\ POP_ASSUM MP_TAC
-  \\ Q.MATCH_ASSUM_RENAME_TAC `TERM defs (Comb (Comb (Const (strlit "=") h2) x1) x2)`
+  \\ Q.MATCH_ASSUM_RENAME_TAC `TERM defs (Comb (Comb (Const (implode "=") h2) x1) x2)`
   \\ REPEAT STRIP_TAC \\ IMP_RES_TAC TERM
   \\ Cases_on `mk_comb (f1,x1) s`
   \\ MP_TAC (mk_comb_thm |> Q.INST [`f`|->`f1`,`a`|->`x1`,`res`|->`q`,`s1`|->`r`])
@@ -1755,7 +1755,7 @@ Proof
   \\ Cases_on `t'` \\ FULL_SIMP_TAC (srw_ss()) [raise_Fail_def]
   \\ Cases_on `t` \\ FULL_SIMP_TAC (srw_ss()) [raise_Fail_def]
   \\ FULL_SIMP_TAC std_ss [st_ex_bind_def]
-  \\ Cases_on `m = (strlit "=")` \\ FULL_SIMP_TAC (srw_ss()) [] \\ SRW_TAC [] []
+  \\ Cases_on `m = (implode "=")` \\ FULL_SIMP_TAC (srw_ss()) [] \\ SRW_TAC [] []
   \\ TRY (
       POP_ASSUM MP_TAC \\
       NTAC 4 BasicProvers.CASE_TAC \\
@@ -1763,7 +1763,7 @@ Proof
       FULL_SIMP_TAC std_ss [] \\
       NO_TAC)
   \\ Q.MATCH_ASSUM_RENAME_TAC
-       `THM defs (Sequent l (Comb (Comb (Const (strlit "=") h) t1) t2))`
+       `THM defs (Sequent l (Comb (Comb (Const (implode "=") h) t1) t2))`
   \\ Cases_on `mk_abs (tm,t1) s` \\ FULL_SIMP_TAC (srw_ss()) []
   \\ MP_TAC (mk_abs_thm |> Q.SPECL [`q`] |> Q.INST [`bvar`|->`tm`,
        `bod`|->`t1`,`s1`|->`r`])
@@ -1843,8 +1843,8 @@ Proof
   \\ STRIP_TAC \\ MP_TAC (type_of_thm |> Q.SPEC `tm`)
   \\ FULL_SIMP_TAC std_ss [] \\ STRIP_TAC \\ FULL_SIMP_TAC std_ss []
   \\ FULL_SIMP_TAC (srw_ss()) [st_ex_bind_def]
-  \\ MP_TAC (mk_type_thm |> Q.SPECL [`strlit"bool"`,`[]`,`s`])
-  \\ Cases_on `mk_type (strlit"bool",[]) s`
+  \\ MP_TAC (mk_type_thm |> Q.SPECL [`implode"bool"`,`[]`,`s`])
+  \\ Cases_on `mk_type (implode"bool",[]) s`
   \\ FULL_SIMP_TAC (srw_ss()) [EVERY_DEF]
   \\ Cases_on `q` \\ FULL_SIMP_TAC (srw_ss()) []
   \\ STRIP_TAC \\ FULL_SIMP_TAC std_ss []
@@ -1873,7 +1873,7 @@ Proof
   \\ SRW_TAC [] [st_ex_bind_def,st_ex_return_def] \\ IMP_RES_TAC THM
   \\ REPEAT STRIP_TAC \\ IMP_RES_TAC TERM
   \\ Q.MATCH_ASSUM_RENAME_TAC `THM defs (Sequent l
-        (Comb (Comb (Const (strlit "=") h1) t1) t2))`
+        (Comb (Comb (Const (implode "=") h1) t1) t2))`
   \\ FULL_SIMP_TAC std_ss [THM_def]
   >> rpt(qpat_x_assum`H |- C`mp_tac) >>
   imp_res_tac term_union_thm >> simp[] >>
@@ -2464,9 +2464,9 @@ Proof
     EVAL_TAC ) >>
   simp[mk_type_def,try_def,otherwise_def,raise_Fail_def,st_ex_return_def,Once st_ex_bind_def] >>
   simp[mk_fun_ty_def] >>
-  `get_type_arity (strlit "fun") s1 = (Success 2, s1)` by (
-    qspecl_then[`(strlit "fun")`,`s1`]mp_tac get_type_arity_thm >>
-    Cases_on`get_type_arity (strlit "fun") s1`>>simp[] >>strip_tac >>
+  `get_type_arity (implode "fun") s1 = (Success 2, s1)` by (
+    qspecl_then[`(implode "fun")`,`s1`]mp_tac get_type_arity_thm >>
+    Cases_on`get_type_arity (implode "fun") s1`>>simp[] >>strip_tac >>
     qunabbrev_tac`s1` >> fs[STATE_def] >>
     imp_res_tac CONTEXT_fun >> rfs[] >>
     METIS_TAC[exc_distinct,exc_11,exc_nchotomy] ) >>
@@ -2601,9 +2601,9 @@ Proof
     simp[MEM_MAP,EXISTS_PROD] >>
     simp[FAPPLY_FUPDATE_THM] >>
     rw[] >> METIS_TAC[]) >>
-  `mk_comb (P,Var (strlit "r") (term_type x)) s2 = (Success (Comb P (Var (strlit "r") (term_type x))), s2)` by (
-    Cases_on`mk_comb (P,Var (strlit "r") (term_type x)) s2` >>
-    MP_TAC (mk_comb_thm |> Q.INST [`f`|->`P`,`a`|->`Var (strlit "r") (term_type x)`,`res`|->`q`,`s1`|->`r`,`s`|->`s2`,`defs`|->`s2.the_context`]) >>
+  `mk_comb (P,Var (implode "r") (term_type x)) s2 = (Success (Comb P (Var (implode "r") (term_type x))), s2)` by (
+    Cases_on`mk_comb (P,Var (implode "r") (term_type x)) s2` >>
+    MP_TAC (mk_comb_thm |> Q.INST [`f`|->`P`,`a`|->`Var (implode "r") (term_type x)`,`res`|->`q`,`s1`|->`r`,`s`|->`s2`,`defs`|->`s2.the_context`]) >>
     impl_tac >- (
       rfs[STATE_def,TERM_Comb,TERM_Var_SIMP] >>
       imp_res_tac term_type ) >>
@@ -2779,8 +2779,8 @@ Theorem new_axiom_thm:
 Proof
   rw[new_axiom_def,st_ex_bind_def] >>
   imp_res_tac type_of_thm >> rw[] >>
-  qspecl_then[`(strlit "bool")`,`[]`,`s`]mp_tac mk_type_thm >>
-  Cases_on`mk_type ((strlit "bool"),[]) s`>>simp[] >>
+  qspecl_then[`(implode "bool")`,`[]`,`s`]mp_tac mk_type_thm >>
+  Cases_on`mk_type ((implode "bool"),[]) s`>>simp[] >>
   Cases_on`q`>>simp[]>>strip_tac>>
   BasicProvers.CASE_TAC >> simp[raise_Fail_def,st_ex_return_def] >>
   simp[get_the_axioms_def,set_the_axioms_def] >>
