candle/standard/semantics/holAxiomsScript.sml
@@ -8,18 +8,18 @@ open preamble holBoolTheory holBoolSyntaxTheory
 
 val _ = new_theory"holAxioms"
 
-Overload A[local] = ``Tyvar (strlit "A")``
-Overload B[local] = ``Tyvar (strlit "B")``
-Overload x[local] = ``Var (strlit "x") A``
-Overload g[local] = ``Var (strlit "f") (Fun A B)``
-Overload B[local] = ``Tyvar (strlit "B")``
-Overload EXx[local] = ``Exists (strlit "x") A``
-Overload x1[local] = ``Var (strlit "x1") A``
-Overload FAx1[local] = ``Forall (strlit "x1") A``
-Overload x2[local] = ``Var (strlit "x2") A``
-Overload FAx2[local] = ``Forall (strlit "x2") A``
-Overload y[local] = ``Var (strlit "y") B``
-Overload FAy[local] = ``Forall (strlit "y") B``
+Overload A[local] = ``Tyvar (implode "A")``
+Overload B[local] = ``Tyvar (implode "B")``
+Overload x[local] = ``Var (implode "x") A``
+Overload g[local] = ``Var (implode "f") (Fun A B)``
+Overload B[local] = ``Tyvar (implode "B")``
+Overload EXx[local] = ``Exists (implode "x") A``
+Overload x1[local] = ``Var (implode "x1") A``
+Overload FAx1[local] = ``Forall (implode "x1") A``
+Overload x2[local] = ``Var (implode "x2") A``
+Overload FAx2[local] = ``Forall (implode "x2") A``
+Overload y[local] = ``Var (implode "y") B``
+Overload FAy[local] = ``Forall (implode "y") B``
 
 val _ = Parse.hide "mem";
 
@@ -49,13 +49,13 @@ Proof
     fs[is_std_sig_def]) >>
   rfs[termsem_def] >>
   rfs[typesem_def] >>
-  qspecl_then[`tmvof v ((strlit "f"),Fun A B)`,`tyvof v (strlit "A")`,`tyvof v (strlit "B")`]mp_tac (UNDISCH in_funspace_abstract) >>
+  qspecl_then[`tmvof v ((implode "f"),Fun A B)`,`tyvof v (implode "A")`,`tyvof v (implode "B")`]mp_tac (UNDISCH in_funspace_abstract) >>
   impl_tac >- ( fs[is_valuation_def,is_type_valuation_def] ) >>
   rw[] >> rw[] >>
   match_mp_tac (UNDISCH abstract_eq) >>
   rw[] >- (
     match_mp_tac (UNDISCH apply_in_rng) >>
-    qexists_tac`tyvof v (strlit "A")` >>
+    qexists_tac`tyvof v (implode "A")` >>
     rw[combinTheory.APPLY_UPDATE_THM] >>
     match_mp_tac (UNDISCH abstract_in_funspace) >>
     rw[] ) >>
@@ -71,7 +71,7 @@ Overload good_select = ``good_select0 ^mem``
 Theorem select_has_model_gen:
    is_set_theory ^mem ⇒
     ∀ctxt.
-      (strlit "@") ∉ FDOM (tmsof ctxt) ∧
+      (implode "@") ∉ FDOM (tmsof ctxt) ∧
       is_implies_sig (tmsof ctxt) ∧
       theory_ok (thyof ctxt)
       ⇒
@@ -81,12 +81,12 @@ Theorem select_has_model_gen:
         good_select select
       ⇒ ∃i'. equal_on (sigof ctxt) i i' ∧
              i' models (thyof (mk_select_ctxt ctxt)) ∧
-             (tmaof i' (strlit "@") =
+             (tmaof i' (implode "@") =
                 (λls. Abstract (Funspace (HD ls) boolset) (HD ls)
                         (λp. select (HD ls) (Holds p))))
 Proof
   rw[good_select_def,models_def,mk_select_ctxt_def,conexts_of_upd_def,is_implies_sig_def,is_implies_interpretation_def] >>
-  qexists_tac`(tyaof i, (strlit "@" =+ λl. Abstract (Funspace (HD l) boolset) (HD l)
+  qexists_tac`(tyaof i, (implode "@" =+ λl. Abstract (Funspace (HD l) boolset) (HD l)
                                       (λp. select (HD l) (Holds p))) (tmaof i))` >>
   imp_res_tac is_std_interpretation_is_type >>
   imp_res_tac typesem_Fun >>
@@ -98,7 +98,7 @@ Proof
       fs[is_interpretation_def,is_term_assignment_def,FEVERY_ALL_FLOOKUP,FLOOKUP_UPDATE] >>
       rw[] >> rw[combinTheory.APPLY_UPDATE_THM] >>
       rw[typesem_def,tyvars_def,STRING_SORT_def,LIST_UNION_def,INORDER_INSERT_def,LIST_INSERT_def] >>
-      fs[is_std_type_assignment_def,mlstringTheory.implode_def] >>
+      fs[is_std_type_assignment_def] >>
       match_mp_tac (UNDISCH abstract_in_funspace) >>
       rw[holds_def] >> fs[is_type_valuation_def]) >>
     conj_tac >- (
@@ -120,8 +120,8 @@ Proof
     simp[satisfies_def] >>
     gen_tac >> strip_tac >>
     qmatch_abbrev_tac`termsem tmsig ii v tm = True` >>
-    `FLOOKUP tmsig (strlit "@") = SOME (Fun (Fun A Bool) A)` by simp[Abbr`tmsig`,FLOOKUP_UPDATE] >>
-    `FLOOKUP tmsig (strlit "==>") = SOME (Fun Bool (Fun Bool Bool))` by simp[Abbr`tmsig`,FLOOKUP_UPDATE] >>
+    `FLOOKUP tmsig (implode "@") = SOME (Fun (Fun A Bool) A)` by simp[Abbr`tmsig`,FLOOKUP_UPDATE] >>
+    `FLOOKUP tmsig (implode "==>") = SOME (Fun Bool (Fun Bool Bool))` by simp[Abbr`tmsig`,FLOOKUP_UPDATE] >>
     imp_res_tac identity_instance >>
     simp[Abbr`tm`,termsem_def] >>
     simp[tyvars_def,STRING_SORT_def,LIST_UNION_def,LIST_INSERT_def,INORDER_INSERT_def] >>
@@ -141,12 +141,12 @@ Proof
     Q.PAT_ABBREV_TAC`fa = tyvof v (implode "A")` >>
     `fx <: fa ∧ fp <: Funspace fa boolset` by (
       fs[is_valuation_def,is_term_valuation_def] >>
-      first_assum(qspecl_then[`strlit "P"`,`Fun A Bool`]mp_tac) >>
-      first_x_assum(qspecl_then[`strlit "x"`,`A`]mp_tac) >>
+      first_assum(qspecl_then[`implode "P"`,`Fun A Bool`]mp_tac) >>
+      first_x_assum(qspecl_then[`implode "x"`,`A`]mp_tac) >>
       imp_res_tac typesem_Bool >>
       simp[type_ok_def,typesem_def] >>
       imp_res_tac theory_ok_sig >>
-      fs[is_std_sig_def,mlstringTheory.implode_def] ) >>
+      fs[is_std_sig_def] ) >>
     `fz <: bs` by (
       unabbrev_all_tac >>
       match_mp_tac (UNDISCH apply_in_rng) >>
@@ -216,7 +216,7 @@ QED
 Theorem select_has_model:
    is_set_theory ^mem ⇒
     ∀ctxt.
-      (strlit "@") ∉ FDOM (tmsof ctxt) ∧
+      (implode "@") ∉ FDOM (tmsof ctxt) ∧
       is_implies_sig (tmsof ctxt) ∧
       theory_ok (thyof ctxt)
       ⇒
@@ -234,8 +234,8 @@ Proof
   metis_tac[good_select_base_select]
 QED
 
-Overload h = ``Var (strlit "f") (Fun Ind Ind)``
-Overload Exh = ``Exists (strlit "f") (Fun Ind Ind)``
+Overload h = ``Var (implode "f") (Fun Ind Ind)``
+Overload Exh = ``Exists (implode "f") (Fun Ind Ind)``
 
 val EVAL_STRING_SORT =
   CONV_TAC (DEPTH_CONV (fn tm => if can (match_term ``STRING_SORT (MAP explode (tyvars X))``) tm
@@ -279,8 +279,8 @@ Theorem infinity_has_model_gen:
    is_set_theory ^mem  ⇒
     ∀ctxt.
       theory_ok (thyof ctxt) ∧
-      DISJOINT (FDOM (tmsof ctxt)) {strlit "ONE_ONE";strlit "ONTO"} ∧
-      (strlit "ind") ∉ FDOM (tysof ctxt) ∧
+      DISJOINT (FDOM (tmsof ctxt)) {implode "ONE_ONE";implode "ONTO"} ∧
+      (implode "ind") ∉ FDOM (tysof ctxt) ∧
       is_implies_sig (tmsof ctxt) ∧
       is_and_sig (tmsof ctxt) ∧
       is_forall_sig (tmsof ctxt) ∧
@@ -297,11 +297,11 @@ Theorem infinity_has_model_gen:
           is_infinite ^mem inf
       ⇒ ∃i'. equal_on (sigof ctxt) i i' ∧
              i' models (thyof (mk_infinity_ctxt ctxt)) ∧
-             (tyaof i' (strlit "ind") [] = inf)
+             (tyaof i' (implode "ind") [] = inf)
 Proof
   rw[models_def,is_implies_sig_def,is_and_sig_def,is_forall_sig_def,is_exists_sig_def,is_not_sig_def,
      is_implies_interpretation_def,is_and_interpretation_def,is_forall_interpretation_def,is_exists_interpretation_def,is_not_interpretation_def] >>
-  `∃ctxt1 p. mk_infinity_ctxt ctxt = (NewAxiom p)::(NewType (strlit "ind") 0)::ctxt1` by simp[mk_infinity_ctxt_def] >>
+  `∃ctxt1 p. mk_infinity_ctxt ctxt = (NewAxiom p)::(NewType (implode "ind") 0)::ctxt1` by simp[mk_infinity_ctxt_def] >>
   `mk_infinity_ctxt ctxt extends ctxt` by (
     match_mp_tac infinity_extends >> simp[] ) >>
   `ctxt1 extends ctxt` by (
@@ -320,8 +320,8 @@ Proof
     fs[mk_infinity_ctxt_def] >> rw[] ) >>
   disch_then(qx_choose_then`i1`strip_assume_tac) >>
   simp[conexts_of_upd_def] >>
-  qexists_tac`(((strlit "ind") =+ (K inf)) (tyaof i1), tmaof i1)` >>
-  `¬(MEM (strlit "ind") (MAP FST (type_list ctxt1)))` by (
+  qexists_tac`(((implode "ind") =+ (K inf)) (tyaof i1), tmaof i1)` >>
+  `¬(MEM (implode "ind") (MAP FST (type_list ctxt1)))` by (
     qpat_x_assum`X = Y::Z`mp_tac >>
     simp[mk_infinity_ctxt_def] >>
     rw[] >> rw[] ) >>
@@ -343,7 +343,7 @@ Proof
         ,FEVERY_ALL_FLOOKUP,combinTheory.APPLY_UPDATE_THM] >>
       rw[] >- metis_tac[] >>
       rfs[FLOOKUP_UPDATE] >>
-      qsuff_tac`typesem ((strlit "ind" =+ K inf) (tyaof i1)) τ v = typesem (tyaof i1) τ v` >- rw[] >>
+      qsuff_tac`typesem ((implode "ind" =+ K inf) (tyaof i1)) τ v = typesem (tyaof i1) τ v` >- rw[] >>
       match_mp_tac typesem_sig >>
       qexists_tac`tysof ctxt1` >>
       conj_tac >- (
@@ -385,12 +385,12 @@ Proof
     ntac 6 (pop_assum kall_tac) >>
     Q.PAT_ABBREV_TAC`tmsig:tmsig = X` >>
     Q.PAT_ABBREV_TAC`int:'U interpretation = X` >>
-    qspecl_then[`tmsig`,`int`,`strlit "/\\"`]mp_tac identity_instance >>
-    qspecl_then[`tmsig`,`int`,`strlit "~"`]mp_tac identity_instance >>
-    qspecl_then[`tmsig`,`int`,`strlit "?"`]mp_tac instance_def >>
-    `(FLOOKUP tmsig (strlit "?") = FLOOKUP (tmsof ctxt) (strlit "?")) ∧
-     (FLOOKUP tmsig (strlit "/\\") = FLOOKUP (tmsof ctxt) (strlit "/\\")) ∧
-     (FLOOKUP tmsig (strlit "~") = FLOOKUP (tmsof ctxt) (strlit "~"))` by (
+    qspecl_then[`tmsig`,`int`,`implode "/\\"`]mp_tac identity_instance >>
+    qspecl_then[`tmsig`,`int`,`implode "~"`]mp_tac identity_instance >>
+    qspecl_then[`tmsig`,`int`,`implode "?"`]mp_tac instance_def >>
+    `(FLOOKUP tmsig (implode "?") = FLOOKUP (tmsof ctxt) (implode "?")) ∧
+     (FLOOKUP tmsig (implode "/\\") = FLOOKUP (tmsof ctxt) (implode "/\\")) ∧
+     (FLOOKUP tmsig (implode "~") = FLOOKUP (tmsof ctxt) (implode "~"))` by (
       simp[Abbr`tmsig`,FLOOKUP_UPDATE] >>
       fs[mk_infinity_ctxt_def] >> rw[] ) >>
     simp[Abbr`tmsig`] >>
@@ -398,23 +398,23 @@ Proof
     simp[REV_ASSOCD] >> disch_then kall_tac >>
     ntac 2 (disch_then kall_tac) >>
     CHANGED_TAC EVAL_STRING_SORT >>
-    simp[typesem_def,combinTheory.APPLY_UPDATE_THM,REV_ASSOCD,mlstringTheory.implode_def] >>
-    `(∀x y. tyaof int (strlit "fun") [x;y] = Funspace x y) ∧
-     (tyaof int (strlit "ind") [] = inf)` by (
+    simp[typesem_def,combinTheory.APPLY_UPDATE_THM,REV_ASSOCD] >>
+    `(∀x y. tyaof int (implode "fun") [x;y] = Funspace x y) ∧
+     (tyaof int (implode "ind") [] = inf)` by (
       simp[Abbr`int`,combinTheory.APPLY_UPDATE_THM] >>
       fs[equal_on_def] >> qx_genl_tac[`a`,`b`] >>
-      last_x_assum (qspec_then`strlit "fun"`mp_tac) >>
+      last_x_assum (qspec_then`implode "fun"`mp_tac) >>
       simp[type_ok_def] >>
       imp_res_tac theory_ok_sig >>
       fs[is_std_sig_def] >>
       imp_res_tac ALOOKUP_MEM >>
       simp[MEM_MAP,EXISTS_PROD,PULL_EXISTS] >>
       fs[is_std_interpretation_def,is_std_type_assignment_def]) >>
-    `(tmaof int (strlit "?") = tmaof i (strlit "?")) ∧
-     (tmaof int (strlit "/\\") = tmaof i (strlit "/\\")) ∧
-     (tmaof int (strlit "!") = tmaof i (strlit "!")) ∧
-     (tmaof int (strlit "==>") = tmaof i (strlit "==>")) ∧
-     (tmaof int (strlit "~") = tmaof i (strlit "~"))` by (
+    `(tmaof int (implode "?") = tmaof i (implode "?")) ∧
+     (tmaof int (implode "/\\") = tmaof i (implode "/\\")) ∧
+     (tmaof int (implode "!") = tmaof i (implode "!")) ∧
+     (tmaof int (implode "==>") = tmaof i (implode "==>")) ∧
+     (tmaof int (implode "~") = tmaof i (implode "~"))` by (
       simp[Abbr`int`] >>
       fs[equal_on_def] >>
       rpt conj_tac >>
@@ -426,24 +426,24 @@ Proof
       imp_res_tac ALOOKUP_MEM >>
       metis_tac[]) >>
     simp[] >>
-    `(FLOOKUP (tmsof ctxt1) (strlit "ONE_ONE") = SOME (Fun (Fun A B) Bool)) ∧
-     (FLOOKUP (tmsof ctxt1) (strlit "ONTO")    = SOME (Fun (Fun A B) Bool))` by (
+    `(FLOOKUP (tmsof ctxt1) (implode "ONE_ONE") = SOME (Fun (Fun A B) Bool)) ∧
+     (FLOOKUP (tmsof ctxt1) (implode "ONTO")    = SOME (Fun (Fun A B) Bool))` by (
       simp[] >>
       fs[mk_infinity_ctxt_def] >>
       rw[] ) >>
-    qspecl_then[`tmsof ctxt1`,`int`,`strlit "ONE_ONE"`]mp_tac instance_def >>
-    qspecl_then[`tmsof ctxt1`,`int`,`strlit "ONTO"`]mp_tac instance_def >>
+    qspecl_then[`tmsof ctxt1`,`int`,`implode "ONE_ONE"`]mp_tac instance_def >>
+    qspecl_then[`tmsof ctxt1`,`int`,`implode "ONTO"`]mp_tac instance_def >>
     simp[] >>
     ntac 2(disch_then(qspec_then`[(Ind,A);(Ind,B)]`strip_assume_tac)) >>
     ntac 2 (pop_assum mp_tac) >>
     simp[REV_ASSOCD] >> ntac 2 (disch_then kall_tac) >>
     EVAL_STRING_SORT >>
-    simp[TYPE_SUBST_def,REV_ASSOCD,typesem_def,mlstringTheory.implode_def] >>
+    simp[TYPE_SUBST_def,REV_ASSOCD,typesem_def] >>
     simp[Abbr`int`] >>
     fs[interprets_def] >>
     first_x_assum(qspec_then`K boolset`mp_tac) >>
     impl_tac >- (simp[is_type_valuation_def,mem_boolset]>>PROVE_TAC[]) >> strip_tac >>
-    first_assum(qspec_then`(strlit "A" =+ (Funspace inf inf)) (K boolset)`mp_tac) >>
+    first_assum(qspec_then`(implode "A" =+ (Funspace inf inf)) (K boolset)`mp_tac) >>
     impl_tac >- (
       simp[is_type_valuation_def,combinTheory.APPLY_UPDATE_THM] >>
       reverse(rw[mem_boolset])>-metis_tac[]>>
@@ -451,7 +451,7 @@ Proof
       match_mp_tac (UNDISCH abstract_in_funspace) >>
       rw[] ) >>
     simp[combinTheory.APPLY_UPDATE_THM] >> disch_then kall_tac >>
-    first_x_assum(qspec_then`(strlit "A" =+ inf) (K boolset)`mp_tac) >>
+    first_x_assum(qspec_then`(implode "A" =+ inf) (K boolset)`mp_tac) >>
     impl_tac >- (
       simp[is_type_valuation_def,combinTheory.APPLY_UPDATE_THM] >>
       rw[mem_boolset]>>
@@ -459,12 +459,12 @@ Proof
     simp[combinTheory.APPLY_UPDATE_THM] >> strip_tac >>
     match_mp_tac apply_abstract_matchable >>
     simp[boolean_in_boolset,boolean_eq_true] >>
-    first_assum(qspec_then`Const (strlit "ONE_ONE") (Fun (Fun A B) Bool) ===
+    first_assum(qspec_then`Const (implode "ONE_ONE") (Fun (Fun A B) Bool) ===
                            Abs g (FAx1 (FAx2 (Implies (Comb g x1 === Comb g x2) (x1 === x2))))`
                 mp_tac) >>
     impl_tac >- ( fs[mk_infinity_ctxt_def] >> rw[] >> EVAL_TAC ) >>
     simp[satisfies_def] >>
-    qabbrev_tac`τ = (strlit "A" =+ inf) ((strlit "B" =+ inf) (K boolset))` >>
+    qabbrev_tac`τ = (implode "A" =+ inf) ((implode "B" =+ inf) (K boolset))` >>
     `is_type_valuation τ` by (
       simp[is_type_valuation_def,Abbr`τ`,combinTheory.APPLY_UPDATE_THM] >>
       rw[] >> metis_tac[boolean_in_boolset] ) >>
@@ -477,11 +477,11 @@ Proof
       imp_res_tac theory_ok_sig >>
       fs[] ) >>
     `is_structure (sigof ctxt1) i1 (τ,σ)` by fs[is_structure_def] >>
-    `(ALOOKUP (const_list ctxt1) (strlit "==>") = ALOOKUP (const_list ctxt) (strlit "==>")) ∧
-     (ALOOKUP (const_list ctxt1) (strlit "!") = ALOOKUP (const_list ctxt) (strlit "!")) ∧
-     (ALOOKUP (const_list ctxt1) (strlit "?") = ALOOKUP (const_list ctxt) (strlit "?")) ∧
-     (ALOOKUP (const_list ctxt1) (strlit "ONE_ONE") = SOME (Fun (Fun A B) Bool)) ∧
-     (ALOOKUP (const_list ctxt1) (strlit "ONTO")    = SOME (Fun (Fun A B) Bool))` by (
+    `(ALOOKUP (const_list ctxt1) (implode "==>") = ALOOKUP (const_list ctxt) (implode "==>")) ∧
+     (ALOOKUP (const_list ctxt1) (implode "!") = ALOOKUP (const_list ctxt) (implode "!")) ∧
+     (ALOOKUP (const_list ctxt1) (implode "?") = ALOOKUP (const_list ctxt) (implode "?")) ∧
+     (ALOOKUP (const_list ctxt1) (implode "ONE_ONE") = SOME (Fun (Fun A B) Bool)) ∧
+     (ALOOKUP (const_list ctxt1) (implode "ONTO")    = SOME (Fun (Fun A B) Bool))` by (
        fs[mk_infinity_ctxt_def] >> rw[] ) >>
     Q.PAT_ABBREV_TAC`eq = X === Y` >>
     `term_ok (sigof ctxt1) eq` by (
@@ -491,13 +491,13 @@ Proof
     simp[Abbr`eq`,SIMP_RULE std_ss [] termsem_equation,boolean_eq_true] >>
     simp[Once termsem_def,identity_instance] >>
     EVAL_STRING_SORT >>
-    `(τ(strlit "A") = inf) ∧ (τ(strlit "B") = inf)` by (
+    `(τ(implode "A") = inf) ∧ (τ(implode "B") = inf)` by (
       simp[Abbr`τ`,combinTheory.APPLY_UPDATE_THM] ) >>
-    simp[mlstringTheory.implode_def] >> disch_then kall_tac >>
-    `(tyaof i1 (strlit "bool") [] = boolset) ∧
-     (∀x y. tyaof i1 (strlit "fun") [x;y] = Funspace x y)` by (
+    simp[] >> disch_then kall_tac >>
+    `(tyaof i1 (implode "bool") [] = boolset) ∧
+     (∀x y. tyaof i1 (implode "fun") [x;y] = Funspace x y)` by (
       fs[is_std_type_assignment_def] ) >>
-    first_assum(qspec_then`Const (strlit "ONTO") (Fun (Fun A B) Bool) ===
+    first_assum(qspec_then`Const (implode "ONTO") (Fun (Fun A B) Bool) ===
                            Abs g (FAy (EXx (y === Comb g x)))`
                 mp_tac) >>
     impl_tac >- ( fs[mk_infinity_ctxt_def] >> rw[] >> EVAL_TAC ) >>
@@ -512,18 +512,18 @@ Proof
     simp[SIMP_RULE std_ss [] termsem_equation,Abbr`eq`,boolean_eq_true] >>
     simp[Once termsem_def,identity_instance] >>
     EVAL_STRING_SORT >>
-    simp[mlstringTheory.implode_def] >> disch_then kall_tac >>
+    simp[] >> disch_then kall_tac >>
     ntac 2 (last_x_assum(qspec_then`τ`mp_tac)) >>
     impl_tac >- rw[] >> strip_tac >>
     impl_tac >- rw[] >> strip_tac >>
     simp[] >>
     simp[termsem_def,identity_instance] >>
-    qspecl_then[`tmsof ctxt1`,`i1`,`strlit "!"`]mp_tac instance_def >>
+    qspecl_then[`tmsof ctxt1`,`i1`,`implode "!"`]mp_tac instance_def >>
     simp[] >>
     disch_then(qspec_then`[B,A]`mp_tac) >>
     simp[REV_ASSOCD] >>
     EVAL_STRING_SORT >>
-    simp[typesem_def,REV_ASSOCD,mlstringTheory.implode_def] >>
+    simp[typesem_def,REV_ASSOCD] >>
     disch_then kall_tac >>
     first_x_assum(qspec_then`τ`mp_tac) >>
     simp[] >> disch_then kall_tac >>
@@ -669,7 +669,7 @@ Proof
     simp[SIMP_RULE std_ss [] termsem_equation,boolean_in_boolset,Abbr`eq`] >>
     rw[boolean_def] >> pop_assum mp_tac >>
     simp[termsem_def,Abbr`tt`,combinTheory.APPLY_UPDATE_THM] >>
-    `Abstract (τ(strlit "B")) (τ(strlit "B")) f ' z = f z` by (
+    `Abstract (τ(implode "B")) (τ(implode "B")) f ' z = f z` by (
       match_mp_tac (UNDISCH apply_abstract) >>
       simp[] >>
       qpat_x_assum`INJ f X Y`mp_tac >>
@@ -682,8 +682,8 @@ Theorem infinity_has_model:
    is_set_theory ^mem ∧ (∃inf. is_infinite ^mem inf) ⇒
     ∀ctxt.
       theory_ok (thyof ctxt) ∧
-      DISJOINT (FDOM (tmsof ctxt)) {strlit"ONE_ONE";strlit"ONTO"} ∧
-      strlit"ind" ∉ FDOM (tysof ctxt) ∧
+      DISJOINT (FDOM (tmsof ctxt)) {implode"ONE_ONE";implode"ONTO"} ∧
+      implode"ind" ∉ FDOM (tysof ctxt) ∧
       is_implies_sig (tmsof ctxt) ∧
       is_and_sig (tmsof ctxt) ∧
       is_forall_sig (tmsof ctxt) ∧
