candle/standard/syntax/holSyntaxExtraScript.sml
@@ -1686,7 +1686,7 @@ Proof
   imp_res_tac term_ok_welltyped >>
   imp_res_tac term_ok_type_ok >>
   fs[is_std_sig_def,type_ok_def] >>
-  qexists_tac`[(typeof s,Tyvar (strlit "A"))]` >>
+  qexists_tac`[(typeof s,Tyvar (implode "A"))]` >>
   rw[holSyntaxLibTheory.REV_ASSOCD_def]
 QED
 
@@ -1705,7 +1705,7 @@ Proof
   fs[is_std_sig_def] >>
   TRY (
     rw[EQ_IMP_THM] >>
-    qexists_tac`[(ty,Tyvar(strlit"A"))]` >>
+    qexists_tac`[(ty,Tyvar(implode"A"))]` >>
     EVAL_TAC >> NO_TAC) >>
   metis_tac[]
 QED
@@ -2766,15 +2766,15 @@ val fresh_term_def = new_specification("fresh_term_def",["fresh_term"],
     conj_tac >- metis_tac[rename_bvars_welltyped] >>
     conj_tac >- (
       match_mp_tac rename_bvars_ACONV >>
-      fs[IN_DISJOINT,MEM_MAP,implode_def] >>
+      fs[IN_DISJOINT,MEM_MAP] >>
       Cases >> simp[] >>
-      metis_tac[explode_implode,implode_def] ) >>
+      metis_tac[explode_implode] ) >>
     qspecl_then[`MAP implode names`,`[]`,`tm`]mp_tac bv_names_rename_bvars >>
     simp[TAKE_LENGTH_ID_rwt] >>
-    fs[IN_DISJOINT,MEM_MAP,implode_def] >>
+    fs[IN_DISJOINT,MEM_MAP] >>
     strip_tac >>
     Cases >> simp[] >>
-    metis_tac[explode_implode,implode_def] ))
+    metis_tac[explode_implode] ))
 
 (* Alternative characterisation of VARIANT, and thereby of VSUBST and INST_CORE.
    Better for evaluation. *)
@@ -2803,17 +2803,17 @@ val variant_def = tDefine "variant" `
   variant avoid v =
     if EXISTS (vfree_in v) avoid then
     case v of
-       Var s ty => variant avoid (Var(s ^ (strlit "'")) ty)
+       Var s ty => variant avoid (Var(s ^ (implode "'")) ty)
     | _ => v else v`
   (WF_REL_TAC `measure (\(avoid,v).
      let n = SUM_SET (BIGUNION (set (MAP (λa. {strlen x + 1 | ∃ty. VFREE_IN (Var x ty) a}) avoid))) in
        n - (case v of Var x ty => strlen x | _ => 0))` >>
-   gen_tac >> Cases >> srw_tac[][strlen_def,strcat_thm,implode_def] >>
+   gen_tac >> Cases >> srw_tac[][strlen_def,strcat_thm] >>
    qsuff_tac`STRLEN s' < n` >- simp[] >>
    simp[Abbr`n`] >> fs[GSYM vfree_in_thm,EXISTS_MEM] >>
    match_mp_tac SUM_SET_IN_LT >>
    qexists_tac`STRLEN s' + 1` >> simp[MEM_MAP,PULL_EXISTS] >>
-   map_every qexists_tac[`e`,`strlit s'`,`ty`] >> simp[] >> rw[] >>
+   map_every qexists_tac[`e`,`implode s'`,`ty`] >> simp[] >> rw[] >>
    qmatch_abbrev_tac`FINITE s` >>
    `s = IMAGE (λ(x,ty). strlen x + 1) {(x,ty) | VFREE_IN (Var x ty) a}` by (
      simp[Abbr`s`,pred_setTheory.EXTENSION,PULL_EXISTS,strlen_def] ) >>
@@ -2849,7 +2849,7 @@ val variant_vsubst_thm = save_thm("variant_vsubst_thm",prove(
   THEN1 (REPEAT STRIP_TAC \\ `SUC m < SUC n` by DECIDE_TAC \\ RES_TAC \\ FULL_SIMP_TAC std_ss [rich_listTheory.REPLICATE_GENLIST]
          \\ FULL_SIMP_TAC std_ss [mlstringTheory.strcat_thm,mlstringTheory.explode_implode])
   \\ FULL_SIMP_TAC (srw_ss()) [rich_listTheory.REPLICATE_GENLIST,GENLIST_CONS]
-  \\ MP_TAC (VARIANT_PRIMES_def |> Q.SPECL [`x`,`explode (name ^ strlit "'")`,`ty`])
+  \\ MP_TAC (VARIANT_PRIMES_def |> Q.SPECL [`x`,`explode (name ^ implode "'")`,`ty`])
   \\ FULL_SIMP_TAC std_ss [GSYM APPEND_ASSOC,APPEND,mlstringTheory.strcat_thm,explode_implode,explode_thm]
   \\ Cases_on `VARIANT_PRIMES x (STRCAT (explode name) "'") (ty) = n`
   \\ FULL_SIMP_TAC std_ss []
@@ -3540,7 +3540,7 @@ Proof
     metis_tac[type_ok_extend,term_ok_type_ok] ) >>
   simp[] >>
   imp_res_tac WELLTYPED_LEMMA >>
-  `name ∉ {strlit "fun";strlit "bool"}` by (
+  `name ∉ {implode "fun";implode "bool"}` by (
     fs[is_std_sig_def] >>
     imp_res_tac ALOOKUP_MEM >>
     fs[MEM_MAP,EXISTS_PROD] >>
@@ -3892,7 +3892,7 @@ val Const_subterm_types_in = Q.prove(
   metis_tac[])
 
 Theorem subterm_typeof_types_in:
-   ∀t1 t2 name args. (Tyapp name args) subtype (typeof t1) ∧ t1 subterm t2 ∧ welltyped t2 ∧ name ≠ (strlit"fun") ⇒
+   ∀t1 t2 name args. (Tyapp name args) subtype (typeof t1) ∧ t1 subterm t2 ∧ welltyped t2 ∧ name ≠ (implode"fun") ⇒
       ∃ty2. Tyapp name args subtype ty2 ∧ ty2 ∈ types_in t2
 Proof
   ho_match_mp_tac term_induction >>
